working on coq proof for the correctness of LEXICAL translator: use a dependent nameless representation

LEXICAL/proof.v
@@ -1,4 +1,4 @@
-Require Import Bool ZArith Arith String List Max.
+Require Import Bool ZArith Arith String List Max Logic.Eqdep_dec.
 Set Implicit Arguments.
 
 Notation "x <- e1 ; e2" :=
@@ -8,303 +8,701 @@ Notation "x <- e1 ; e2" :=
     end)
 (right associativity, at level 60).
 
-Lemma option_eq {T : Type} (p q : T) : Some p = Some q -> p = q.
-    congruence.
-Qed.
-
 Module Proc.
-  Inductive expression : Set :=
-  | Const : nat -> expression
-  | Diff : expression -> expression -> expression
-  | IsZero : expression -> expression
-  | If : expression -> expression -> expression -> expression
-  | Var : string -> expression
-  | Let : string -> expression -> expression -> expression
-  | Proc : string -> expression -> expression
-  | Call : expression -> expression -> expression
-  .
+    Inductive expression : Set :=
+    | Const : nat -> expression
+    | Diff : expression -> expression -> expression
+    | IsZero : expression -> expression
+    | If : expression -> expression -> expression -> expression
+    | Var : string -> expression
+    | Let : string -> expression -> expression -> expression
+    | Proc : string -> expression -> expression
+    | Call : expression -> expression -> expression
+    .
 
-  Inductive expval : Set :=
-  | Num : Z -> expval
-  | Bool : bool -> expval
-  | Clo : string -> expression -> list (string * expval) -> expval
-  .
+    Inductive expval : Set :=
+    | Num : Z -> expval
+    | Bool : bool -> expval
+    | Clo : string -> expression -> environment -> expval
 
-  Definition environment := list (string * expval).
-  Definition empty_env : environment := nil.
-  Definition extend_env (x : string) (v : expval) (env : environment) := (x, v) :: env.
+    with environment : Set :=
+    | Empty : environment
+    | Extend : string -> expval -> environment -> environment
+    .
 
-  Fixpoint assoc (x : string) (env : environment) : option expval :=
-      match env with
-      | nil => None
-      | (y, v) :: saved_env => if string_dec x y then Some v else assoc x saved_env
-      end.
+    Scheme expval_mut := Induction for expval Sort Prop
+    with environment_mut := Induction for environment Sort Prop.
 
-  Inductive value_of_rel : expression -> environment -> expval -> Prop :=
-  | VConst : forall num env, value_of_rel (Const num) env (Num (Z.of_nat num))
-  | VDiff : forall exp1 exp2 num1 num2 env, value_of_rel exp1 env (Num num1) -> value_of_rel exp2 env (Num num2) -> value_of_rel (Diff exp1 exp2) env (Num (num1 - num2))
-  | VIsZero : forall exp1 num1 env, value_of_rel exp1 env (Num num1) -> value_of_rel (IsZero exp1) env (Bool (Z.eqb num1 0))
-  | VIfTrue : forall exp1 exp2 exp3 val2 env, value_of_rel exp1 env (Bool true) -> value_of_rel exp2 env val2 -> value_of_rel (If exp1 exp2 exp3) env val2
-  | VIfFalse : forall exp1 exp2 exp3 val3 env, value_of_rel exp1 env (Bool false) -> value_of_rel exp3 env val3 -> value_of_rel (If exp1 exp2 exp3) env val3
-  | VVar : forall var env val, assoc var env = Some val -> value_of_rel (Var var) env val
-  | VLet : forall var exp1 body env val1 valb, value_of_rel exp1 env val1 -> value_of_rel body (extend_env var val1 env) valb -> value_of_rel (Let var exp1 body) env valb
-  | VProc : forall var body env, value_of_rel (Proc var body) env (Clo var body env)
-  | VCall : forall rator rand env var body saved_env rand_val valb, value_of_rel rator env (Clo var body saved_env) -> value_of_rel rand env rand_val -> value_of_rel body (extend_env var rand_val saved_env) valb -> value_of_rel (Call rator rand) env valb
-  .
+    Fixpoint assoc_error (x : string) (env : environment) : option expval :=
+        match env with
+        | Empty => None
+        | Extend y val saved_env => if string_dec x y then Some val else assoc_error x saved_env
+        end.
+
+    Inductive value_of_rel : expression -> environment -> expval -> Prop :=
+    | VConst : forall num env, value_of_rel (Const num) env (Num (Z.of_nat num))
+    | VDiff : forall exp1 exp2 num1 num2 env, value_of_rel exp1 env (Num num1) -> value_of_rel exp2 env (Num num2) -> value_of_rel (Diff exp1 exp2) env (Num (num1 - num2))
+    | VIsZero : forall exp1 num1 env, value_of_rel exp1 env (Num num1) -> value_of_rel (IsZero exp1) env (Bool (Z.eqb num1 0))
+    | VIfTrue : forall exp1 exp2 exp3 val2 env, value_of_rel exp1 env (Bool true) -> value_of_rel exp2 env val2 -> value_of_rel (If exp1 exp2 exp3) env val2
+    | VIfFalse : forall exp1 exp2 exp3 val3 env, value_of_rel exp1 env (Bool false) -> value_of_rel exp3 env val3 -> value_of_rel (If exp1 exp2 exp3) env val3
+    | VVar : forall var env val, assoc_error var env = Some val -> value_of_rel (Var var) env val
+    | VLet : forall var exp1 body env val1 valb, value_of_rel exp1 env val1 -> value_of_rel body (Extend var val1 env) valb -> value_of_rel (Let var exp1 body) env valb
+    | VProc : forall var body env, value_of_rel (Proc var body) env (Clo var body env)
+    | VCall : forall rator rand env var body saved_env rand_val valb, value_of_rel rator env (Clo var body saved_env) -> value_of_rel rand env rand_val -> value_of_rel body (Extend var rand_val saved_env) valb -> value_of_rel (Call rator rand) env valb
+    .
 End Proc.
 
 Module Lexical.
-  Inductive expression : Set :=
-  | Const : nat -> expression
-  | Diff : expression -> expression -> expression
-  | IsZero : expression -> expression
-  | If : expression -> expression -> expression -> expression
-  | Var : nat -> expression
-  | Let : expression -> expression -> expression
-  | Proc : expression -> expression
-  | Call : expression -> expression -> expression
-  .
+    Inductive expression : nat -> Set :=
+    | Const : forall ctx, nat -> expression ctx
+    | Diff : forall ctx, expression ctx -> expression ctx -> expression ctx
+    | IsZero : forall ctx, expression ctx -> expression ctx
+    | If : forall ctx, expression ctx -> expression ctx -> expression ctx -> expression ctx
+    | Var : forall ctx n, n < ctx -> expression ctx
+    | Let : forall ctx, expression ctx -> expression (S ctx) -> expression ctx
+    | Proc : forall ctx, expression (S ctx) -> expression ctx
+    | Call : forall ctx, expression ctx -> expression ctx -> expression ctx
+    .
 
-  Inductive expval : Set :=
-  | Num : Z -> expval
-  | Bool : bool -> expval
-  | Clo : expression -> list expval -> expval
-  .
+    Inductive expval : Set :=
+    | Num : Z -> expval
+    | Bool : bool -> expval
+    | Clo : forall ctx, expression (S ctx) -> environment ctx -> expval
 
-  Definition environment := list expval.
-  Definition empty_env : environment := nil.
-  Definition extend_env (v : expval) (env : environment) := v :: env.
+    with environment : nat -> Set :=
+    | Empty : environment O
+    | Extend : forall ctx, expval -> environment ctx -> environment (S ctx)
+    .
 
-  Inductive value_of_rel : expression -> environment -> expval -> Prop :=
-  | VConst : forall num env, value_of_rel (Const num) env (Num (Z.of_nat num))
-  | VDiff : forall exp1 exp2 num1 num2 env, value_of_rel exp1 env (Num num1) -> value_of_rel exp2 env (Num num2) -> value_of_rel (Diff exp1 exp2) env (Num (num1 - num2))
-  | VIsZero : forall exp1 num1 env, value_of_rel exp1 env (Num num1) -> value_of_rel (IsZero exp1) env (Bool (Z.eqb num1 0))
-  | VIfTrue : forall exp1 exp2 exp3 val2 env, value_of_rel exp1 env (Bool true) -> value_of_rel exp2 env val2 -> value_of_rel (If exp1 exp2 exp3) env val2
-  | VIfFalse : forall exp1 exp2 exp3 val3 env, value_of_rel exp1 env (Bool false) -> value_of_rel exp3 env val3 -> value_of_rel (If exp1 exp2 exp3) env val3
-  | VVar : forall n env val, nth_error env n = value val -> value_of_rel (Var n) env val
-  | VLet : forall exp1 body env val1 valb, value_of_rel exp1 env val1 -> value_of_rel body (extend_env val1 env) valb -> value_of_rel (Let exp1 body) env valb
-  | VProc : forall body env, value_of_rel (Proc body) env (Clo body env)
-  | VCall : forall rator rand env body saved_env rand_val valb, value_of_rel rator env (Clo body saved_env) -> value_of_rel rand env rand_val -> value_of_rel body (extend_env rand_val saved_env) valb -> value_of_rel (Call rator rand) env valb
-  .
+    Scheme expval_mut := Induction for expval Sort Prop
+    with environment_mut := Induction for environment Sort Prop.
 
-  Function value_of (exp : expression) (env : environment) (fuel : nat) : option expval :=
-      match fuel with
-      | O => None
-      | S fuel' =>
-              match exp with
-              | Const num => Some (Num (Z.of_nat num))
-              | Diff exp1 exp2 =>
-                      val1 <- value_of exp1 env fuel';
-                      val2 <- value_of exp2 env fuel';
-                      match (val1, val2) with
-                      | (Num num1, Num num2) => Some (Num (num1 - num2))
-                      | _ => None
-                      end
-              | IsZero exp1 =>
-                      val1 <- value_of exp1 env fuel';
-                      match val1 with
-                      | Num num1 => Some (Bool (Z.eqb num1 0))
-                      | _ => None
-                      end
-              | If exp1 exp2 exp3 =>
-                      val1 <- value_of exp1 env fuel';
-                      match val1 with
-                      | Bool true => value_of exp2 env fuel'
-                      | Bool false => value_of exp3 env fuel'
-                      | _ => None
-                      end
-              | Var n =>
-                      match nth_error env n with
-                      | value val => Some val
-                      | error => None
-                      end
-              | Let exp1 body =>
-                      val1 <- value_of exp1 env fuel';
-                      value_of body (extend_env val1 env) fuel'
-              | Proc body => Some (Clo body env)
-              | Call rator rand =>
-                      rator_val <- value_of rator env fuel';
-                      match rator_val with
-                      | Clo body saved_env =>
-                              rand_val <- value_of rand env fuel';
-                              value_of body (extend_env rand_val saved_env) fuel'
-                      | _ => None
-                      end
-              end
-      end.
+    Lemma nltz : forall n, n < O -> False.
+        intro; omega.
+    Qed.
 
-  Hint Constructors value_of_rel.
+    Fixpoint nth {ctx : nat} (n : nat) (env : environment ctx) : n < ctx -> expval :=
+        match env in (environment ctx) with
+        | Empty => fun pf => match nltz pf with end
+        | Extend _ val saved_env =>
+                match n with
+                | O => fun _ => val
+                | S _ => fun pf => nth saved_env (lt_S_n _ _ pf)
+                end
+        end.
 
-  Theorem value_of_soundness : forall exp env val, (exists fuel, value_of exp env fuel = Some val) -> value_of_rel exp env val.
-      intros.
-      destruct 0 as [ fuel ? ].
-      generalize dependent val.
-      generalize dependent env.
-      generalize dependent exp.
-      induction fuel; intros; try discriminate; destruct exp;
-      match goal with
-      | [ H : value_of _ _ _ = _ |- _ ] => simpl in H
-      end;
-      repeat (try match goal with
-                  | [ _ : context[match value_of ?EXP ?ENV ?FUEL with Some _ => _ | None => _ end] |- _ ] => destruct (value_of EXP ENV FUEL) eqn:?; try discriminate
-                  | [ _ : context[match ?VAL with Num _ => _ | Bool _ => _ | Clo _ _ => _ end] |- _ ] => destruct VAL; try discriminate
-                  | [ _ : context[if ?B then _ else _] |- _ ] => destruct B
-                  | [ _ : context[match nth_error ?ENV ?N with value _ => _ | error => _ end] |- _ ] => destruct (nth_error ENV N) eqn:?; try discriminate
-                  | [ H : Some _ = Some _ |- _ ] => apply option_eq in H; try (rewrite <- H)
-                  end;
-              eauto).
-  Qed.
+    Inductive value_of_rel: forall ctx, expression ctx -> environment ctx -> expval -> Prop :=
+    | VConst : forall ctx num env, value_of_rel (Const ctx num) env (Num (Z.of_nat num))
+    | VDiff : forall ctx (exp1 : expression ctx) exp2 num1 num2 env, value_of_rel exp1 env (Num num1) -> value_of_rel exp2 env (Num num2) -> value_of_rel (Diff exp1 exp2) env (Num (num1 - num2))
+    | VIsZero : forall ctx (exp1 : expression ctx) num1 env, value_of_rel exp1 env (Num num1) -> value_of_rel (IsZero exp1) env (Bool (Z.eqb num1 0))
+    | VIfTrue : forall ctx (exp1 : expression ctx) exp2 exp3 val2 env, value_of_rel exp1 env (Bool true) -> value_of_rel exp2 env val2 -> value_of_rel (If exp1 exp2 exp3) env val2
+    | VIfFalse : forall ctx (exp1 : expression ctx) exp2 exp3 val3 env, value_of_rel exp1 env (Bool false) -> value_of_rel exp3 env val3 -> value_of_rel (If exp1 exp2 exp3) env val3
+    | VVar : forall ctx n (pf : n < ctx) env val, nth env pf = val -> value_of_rel (Var pf) env val
+    | VLet : forall ctx (exp1 : expression ctx) body env val1 val, value_of_rel exp1 env val1 -> value_of_rel body (Extend val1 env) val -> value_of_rel (Let exp1 body) env val
+    | VProc : forall ctx (body : expression (S ctx)) env, value_of_rel (Proc body) env (Clo body env)
+    | VCall : forall ctx (rator : expression ctx) rand env ctx' (body : expression (S ctx')) saved_env rand_val val, value_of_rel rator env (Clo body saved_env) -> value_of_rel rand env rand_val -> value_of_rel body (Extend rand_val saved_env) val -> value_of_rel (Call rator rand) env val
+    .
 
-  Lemma fuel_incr : forall fuel exp env val, value_of exp env fuel = Some val -> value_of exp env (S fuel) = Some val.
-      induction fuel; intros; try discriminate; destruct exp;
-      match goal with
-      | [ H : value_of _ _ _ = _ |- _ ] => simpl in H
-      end;
-      rewrite value_of_equation;
-      repeat (try match goal with
-                  | [ _ : context[match value_of ?EXP ?ENV ?FUEL with Some _ => _ | None => _ end] |- _ ] => destruct (value_of EXP ENV FUEL) eqn:?; try discriminate
-                  | [ _ : context[match ?VAL with Num _ => _ | Bool _ => _ | Clo _ _ => _ end] |- _ ] => destruct VAL; try discriminate
-                  | [ _ : context[if ?B then _ else _] |- _ ] => destruct B
-                  | [ IH : forall _, _, H : value_of ?EXP ?ENV ?FUEL = Some ?VAL |- context[match value_of ?EXP ?ENV (S ?FUEL) with Some _ => _ | None => _ end] ] => assert (T := IH EXP ENV VAL); apply T in H; clear T; try (rewrite -> H; clear H)
-                  end;
-              eauto).
-  Qed.
+    Lemma value_of_rel_diff_inversion : forall ctx (exp1 : expression ctx) exp2 env val, value_of_rel (Diff exp1 exp2) env val -> exists num1 num2, value_of_rel exp1 env (Num num1) /\ value_of_rel exp2 env (Num num2) /\ val = Num (num1 - num2).
+        Hint Resolve eq_nat_dec.
+        intros.
+        inversion H.
+        apply inj_pair2_eq_dec in H0; auto.
+        apply inj_pair2_eq_dec in H1; auto.
+        apply inj_pair2_eq_dec in H3; auto.
+        subst.
+        eauto.
+    Qed.
 
-  Lemma fuel_order : forall exp env val fuel fuel', value_of exp env fuel = Some val -> fuel <= fuel' -> value_of exp env fuel' = Some val.
-      Hint Resolve fuel_incr.
-      induction 2; auto.
-  Qed.
+    Lemma value_of_rel_is_zero_inversion : forall ctx (exp1 : expression ctx) env val, value_of_rel (IsZero exp1) env val -> exists num1, value_of_rel exp1 env (Num num1) /\ val = Bool (Z.eqb num1 0).
+        Hint Resolve eq_nat_dec.
+        intros.
+        inversion H.
+        apply inj_pair2_eq_dec in H0; auto.
+        apply inj_pair2_eq_dec in H2; auto.
+        subst.
+        eauto.
+    Qed.
 
-  Lemma le_max_1 : forall a b c, a <= max (max a b) c.
-      intros.
-      assert (max a (max b c) = max (max a b) c).
-      apply max_assoc.
-      rewrite <- H.
-      apply le_max_l.
-  Qed.
+    Lemma value_of_rel_if_inversion : forall ctx (exp1 : expression ctx) exp2 exp3 env val, value_of_rel (If exp1 exp2 exp3) env val -> (value_of_rel exp1 env (Bool true) /\ value_of_rel exp2 env val) \/ (value_of_rel exp1 env (Bool false) /\ value_of_rel exp3 env val).
+        Hint Resolve eq_nat_dec.
+        intros.
+        inversion H.
+            left.
+            apply inj_pair2_eq_dec in H0; auto.
+            apply inj_pair2_eq_dec in H1; auto.
+            apply inj_pair2_eq_dec in H5; auto.
+            subst.
+            auto.
 
-  Lemma le_max_2 : forall a b c, b <= max (max a b) c.
-      intros.
-      assert (b <= max a b).
-      apply le_max_r.
-      assert (max a b <= max (max a b) c).
-      apply le_max_l.
-      omega.
-  Qed.
+            right.
+            apply inj_pair2_eq_dec in H0; auto.
+            apply inj_pair2_eq_dec in H4; auto.
+            apply inj_pair2_eq_dec in H5; auto.
+            subst.
+            auto.
+    Qed.
 
-  Lemma le_max_3 : forall a b c, c <= max (max a b) c.
-      intros.
-      apply le_max_r.
-  Qed.
+    Lemma value_of_rel_let_inversion : forall ctx (exp1 : expression ctx) body env val, value_of_rel (Let exp1 body) env val -> exists val1, value_of_rel exp1 env val1 /\ value_of_rel body (Extend val1 env) val.
+        Hint Resolve eq_nat_dec.
+        intros.
+        inversion H.
+        apply inj_pair2_eq_dec in H0; auto.
+        apply inj_pair2_eq_dec in H1; auto.
+        apply inj_pair2_eq_dec in H3; auto.
+        subst.
+        eauto.
+    Qed.
 
-  Theorem value_of_completeness : forall exp env val, value_of_rel exp env val -> exists fuel, value_of exp env fuel = Some val.
-      Hint Resolve le_max_l le_max_r le_max_1 le_max_2 le_max_3.
-      induction 1;
-      match goal with
-      | [ IH1 : exists _, _, IH2 : exists _, _, IH3 : exists _, _ |- _ ] => destruct IH1 as [ fuel1 ? ]; destruct IH2 as [ fuel2 ? ]; destruct IH3 as [ fuel3 ? ]; exists (S (max (max fuel1 fuel2) fuel3))
-      | [ IH1 : exists _, _, IH2 : exists _, _ |- _ ] => destruct IH1 as [ fuel1 ? ]; destruct IH2 as [ fuel2 ? ]; exists (S (max fuel1 fuel2))
-      | [ IH1 : exists _, _ |- _ ] => destruct IH1 as [ fuel1 ? ]; exists (S fuel1)
-      | [ |- _ ] => exists (S O)
-      end;
-      eauto;
-      rewrite value_of_equation;
-      repeat (try match goal with
-                  | [ H : value_of ?EXP ?ENV ?FUEL1 = _ |- context[value_of ?EXP ?ENV ?FUEL2] ] => apply fuel_order with (fuel' := FUEL2) in H; auto; try (rewrite -> H; clear H)
-                  | [ H : nth_error ?ENV ?N = _ |- context[nth_error ?ENV ?N] ] => destruct (nth_error ENV N)
-                  end;
-              eauto).
-  Qed.
+    Lemma value_of_rel_var_inversion : forall ctx n (pf : n < ctx) env val, value_of_rel (Var pf) env val -> exists (pf : n < ctx), nth env pf = val.
+        Hint Resolve eq_nat_dec.
+        intros.
+        inversion H.
+        apply inj_pair2_eq_dec in H2; auto.
+        subst.
+        eauto.
+    Qed.
 
-  Theorem value_of_correctness : forall exp env val, (exists fuel, value_of exp env fuel = Some val) <-> value_of_rel exp env val.
-      Hint Resolve value_of_soundness value_of_completeness.
-      intros; split; auto.
-  Qed.
+    Lemma value_of_rel_proc_inversion : forall ctx (body : expression (S ctx)) env val, value_of_rel (Proc body) env val -> val = Clo body env.
+        Hint Resolve eq_nat_dec.
+        intros.
+        inversion H.
+        apply inj_pair2_eq_dec in H2; auto.
+        apply inj_pair2_eq_dec in H3; auto.
+        subst.
+        auto.
+    Qed.
+
+    Lemma value_of_rel_call_inversion : forall ctx (rator : expression ctx) rand env val, value_of_rel (Call rator rand) env val -> exists ctx' (body : expression (S ctx')) saved_env rand_val, value_of_rel rator env (Clo body saved_env) /\ value_of_rel rand env rand_val /\ value_of_rel body (Extend rand_val saved_env ) val.
+        Hint Resolve eq_nat_dec.
+        intros.
+        inversion H.
+        apply inj_pair2_eq_dec in H0; auto.
+        apply inj_pair2_eq_dec in H1; auto.
+        apply inj_pair2_eq_dec in H2; auto.
+        subst.
+        exists ctx'.
+        exists body.
+        eauto.
+    Qed.
+
+    Inductive exp_equiv : forall ctx ctx', expression ctx -> expression ctx' -> Prop :=
+    | EQConst : forall ctx ctx' num num', ctx = ctx' -> num = num' -> exp_equiv (Const ctx num) (Const ctx' num')
+    | EQDiff : forall ctx ctx' (exp1 : expression ctx) (exp1' : expression ctx') exp2 exp2', exp_equiv exp1 exp1' -> exp_equiv exp2 exp2' -> exp_equiv (Diff exp1 exp2) (Diff exp1' exp2')
+    | EQIsZero : forall ctx ctx' (exp1 : expression ctx) (exp1' : expression ctx'), exp_equiv exp1 exp1' -> exp_equiv (IsZero exp1) (IsZero exp1')
+    | EQIf : forall ctx ctx' (exp1 : expression ctx) (exp1' : expression ctx') exp2 exp2' exp3 exp3', exp_equiv exp1 exp1' -> exp_equiv exp2 exp2' -> exp_equiv exp3 exp3' -> exp_equiv (If exp1 exp2 exp3) (If exp1' exp2' exp3')
+    | EQLet : forall ctx ctx' (exp1 : expression ctx) (exp1' : expression ctx') body body', exp_equiv exp1 exp1' -> exp_equiv body body' -> exp_equiv (Let exp1 body) (Let exp1' body')
+    | EQVar : forall ctx ctx' n n' (pf : n < ctx) (pf' : n' < ctx'), ctx = ctx' -> n = n' -> exp_equiv (Var pf) (Var pf')
+    | EQProc : forall ctx ctx' (body : expression (S ctx)) (body' : expression (S ctx')), exp_equiv body body' -> exp_equiv (Proc body) (Proc body')
+    | EQCall : forall ctx ctx' (rator : expression ctx) (rator' : expression ctx') rand rand', exp_equiv rator rator' -> exp_equiv rand rand' -> exp_equiv (Call rator rand) (Call rator' rand')
+    .
+
+    Inductive expval_equiv : expval -> expval -> Prop :=
+    | EQNum : forall num num', num = num' -> expval_equiv (Num num) (Num num')
+    | EQBool : forall bool bool', bool = bool' -> expval_equiv (Bool bool) (Bool bool')
+    | EQClo : forall ctx ctx' (body : expression (S ctx)) (body' : expression (S ctx')) saved_env saved_env', exp_equiv body body' -> env_equiv saved_env saved_env' -> expval_equiv (Clo body saved_env) (Clo body' saved_env')
+
+    with env_equiv : forall ctx ctx', environment ctx -> environment ctx' -> Prop :=
+    | EQEmpty : env_equiv Empty Empty
+    | EQExtend : forall ctx ctx' (saved_env : environment ctx) (saved_env' : environment ctx') val val', expval_equiv val val' -> env_equiv saved_env saved_env' -> env_equiv (Extend val saved_env) (Extend val' saved_env')
+    .
+
+    Hint Constructors exp_equiv expval_equiv env_equiv.
+
+    Lemma exp_equiv_refl : forall ctx (exp : expression ctx), exp_equiv exp exp.
+        induction exp; eauto.
+    Qed.
+
+    Lemma exp_equiv_comm : forall ctx ctx' (exp : expression ctx) (exp' : expression ctx'), exp_equiv exp exp' -> exp_equiv exp' exp.
+        intros.
+        induction H; auto.
+    Qed.
+
+    Lemma exp_equiv_tran : forall ctx ctx' ctx'' (exp : expression ctx) (exp' : expression ctx') (exp'' : expression ctx''), exp_equiv exp exp' -> exp_equiv exp' exp'' -> exp_equiv exp exp''.
+    Admitted.
+
+    Lemma exp_equiv_const_inversion : forall ctx (exp : expression ctx) ctx' num', exp_equiv exp (Const ctx' num') -> exists num, ctx = ctx' /\ num = num' /\ exp = Const ctx num.
+        Hint Resolve eq_nat_dec.
+        intros.
+        inversion H.
+        apply inj_pair2_eq_dec in H0; auto.
+        eauto.
+    Qed.
+
+    Lemma exp_equiv_diff_inversion : forall ctx ctx' (exp : expression ctx) (exp1' : expression ctx') exp2', exp_equiv exp (Diff exp1' exp2') -> exists exp1 exp2, exp_equiv exp1 exp1' /\ exp_equiv exp2 exp2' /\ exp = Diff exp1 exp2.
+        Hint Resolve eq_nat_dec.
+        intros.
+        inversion H.
+        apply inj_pair2_eq_dec in H0; auto.
+        apply inj_pair2_eq_dec in H1; auto.
+        apply inj_pair2_eq_dec in H4; auto.
+        subst.
+        eauto.
+    Qed.
+
+    Lemma exp_equiv_var_inversion : forall ctx (exp : expression ctx) ctx' n' (pf' : n' < ctx'), exp_equiv exp (Var pf') -> exists n (pf : n < ctx), ctx = ctx' /\ n = n' /\ exp = Var pf.
+        Hint Resolve eq_nat_dec.
+        intros.
+        inversion H.
+        apply inj_pair2_eq_dec in H0; auto.
+        subst.
+        eauto.
+    Qed.
+
+    Lemma expval_equiv_refl : forall val, expval_equiv val val
+    with env_equiv_refl : forall env, expval_equiv env env.
+    Admitted.
+
+    Fixpoint value_of {ctx : nat} (fuel : nat) (exp : expression ctx) : environment ctx -> option expval :=
+        match fuel with
+        | O => fun _ => None
+        | S fuel' =>
+                match exp with
+                | Const _ num => fun _ => Some (Num (Z.of_nat num))
+                | Diff _ exp1 exp2 => fun env =>
+                        val1 <- value_of fuel' exp1 env;
+                        val2 <- value_of fuel' exp2 env;
+                        match (val1, val2) with
+                        | (Num num1, Num num2) => Some (Num (num1 - num2))
+                        | _ => None
+                        end
+                | IsZero _ exp1 => fun env =>
+                        val1 <- value_of fuel' exp1 env;
+                        match val1 with
+                        | Num num1 => Some (Bool (Z.eqb num1 0))
+                        | _ => None
+                        end
+                | If _ exp1 exp2 exp3 => fun env =>
+                        val1 <- value_of fuel' exp1 env;
+                        match val1 with
+                        | Bool true => value_of fuel' exp2 env
+                        | Bool false => value_of fuel' exp3 env
+                        | _ => None
+                        end
+                | Var _ _ pf => fun env => Some (nth env pf)
+                | Let _ exp1 body => fun env =>
+                        val1 <- value_of fuel' exp1 env;
+                        value_of fuel' body (Extend val1 env)
+                | Proc _ body => fun env => Some (Clo body env)
+                | Call _ rator rand => fun env =>
+                        rator_val <- value_of fuel' rator env;
+                        match rator_val with
+                        | Clo _ body saved_env =>
+                                rand_val <- value_of fuel' rand env;
+                                value_of fuel' body (Extend rand_val saved_env)
+                        | _ => None
+                        end
+                end
+        end.
+
+    Lemma value_of_diff_equation : forall fuel ctx (exp1 : expression ctx) exp2 env num1 num2, value_of fuel exp1 env = Some (Num num1) -> value_of fuel exp2 env = Some (Num num2) -> value_of (S fuel) (Diff exp1 exp2) env = Some (Num (num1 - num2)).
+        intros.
+        simpl.
+        rewrite -> H.
+        rewrite -> H0.
+        trivial.
+    Qed.
+
+    Lemma value_of_is_zero_equation : forall fuel ctx (exp1 : expression ctx) env num1, value_of fuel exp1 env = Some (Num num1) -> value_of (S fuel) (IsZero exp1) env = Some (Bool (Z.eqb num1 0)).
+        intros.
+        simpl.
+        rewrite -> H.
+        trivial.
+    Qed.
+
+    Lemma value_of_if_true_equation : forall fuel ctx (exp1 : expression ctx) exp2 exp3 env val, value_of fuel exp1 env = Some (Bool true) -> value_of fuel exp2 env = Some val -> value_of (S fuel) (If exp1 exp2 exp3) env = Some val.
+        intros.
+        simpl.
+        rewrite -> H.
+        trivial.
+    Qed.
+
+    Lemma value_of_if_false_equation : forall fuel ctx (exp1 : expression ctx) exp2 exp3 env val, value_of fuel exp1 env = Some (Bool false) -> value_of fuel exp3 env = Some val -> value_of (S fuel) (If exp1 exp2 exp3) env = Some val.
+        intros.
+        simpl.
+        rewrite -> H.
+        trivial.
+    Qed.
+
+    Lemma value_of_var_equation : forall fuel ctx (env : environment ctx) n (pf : n < ctx) val, nth env pf = val -> value_of (S fuel) (Var pf) env = Some val.
+        intros.
+        simpl.
+        rewrite -> H.
+        trivial.
+    Qed.
+
+    Lemma value_of_let_equation : forall fuel ctx (exp1 : expression ctx) body env val1 val, value_of fuel exp1 env = Some val1 -> value_of fuel body (Extend val1 env) = Some val -> value_of (S fuel) (Let exp1 body) env = Some val.
+        intros.
+        simpl.
+        rewrite -> H.
+        trivial.
+    Qed.
+
+    Lemma value_of_call_equation : forall fuel ctx (rator : expression ctx) rand env rand_val val ctx' (body : expression (S ctx')) saved_env, value_of fuel rator env = Some (Clo body saved_env) -> value_of fuel rand env = Some rand_val -> value_of fuel body (Extend rand_val saved_env) = Some val -> value_of (S fuel) (Call rator rand) env = Some val.
+        intros.
+        simpl.
+        rewrite -> H.
+        rewrite -> H0.
+        trivial.
+    Qed.
+
+    Hint Resolve value_of_diff_equation value_of_is_zero_equation value_of_if_true_equation value_of_if_false_equation value_of_var_equation value_of_let_equation value_of_call_equation.
+    Hint Constructors value_of_rel.
+
+    Theorem value_of_soundness : forall ctx (exp : expression ctx) env val, (exists fuel, value_of fuel exp env = Some val) -> value_of_rel exp env val.
+        intros.
+        destruct 0 as [ fuel ? ].
+        generalize dependent ctx.
+        generalize dependent val.
+        induction fuel; intros; try discriminate; destruct exp;
+        match goal with
+        | [ H : value_of _ _ _ = _ |- _ ] => simpl in H
+        end;
+        repeat (try match goal with
+                    | [ _ : context[match value_of ?FUEL ?EXP ?ENV with Some _ => _ | None => _ end] |- _ ] => destruct (value_of FUEL EXP ENV) eqn:?; try discriminate
+                    | [ _ : context[match ?VAL with Num _ => _ | Bool _ => _ | Clo _ _ _ => _ end] |- _ ] => destruct VAL; try discriminate
+                    | [ _ : context[if ?B then _ else _] |- _ ] => destruct B
+                    | [ H : Some _ = Some _ |- _ ] => inversion H; subst
+                    end;
+                eauto).
+    Qed.
+
+    Lemma fuel_incr : forall fuel ctx (exp : expression ctx) env val, value_of fuel exp env = Some val -> value_of (S fuel) exp env = Some val.
+        induction fuel; intros; try discriminate; destruct exp;
+        match goal with
+        | [ H : value_of _ _ _ = _ |- _ ] => simpl in H
+        end;
+        repeat (try match goal with
+                    | [ _ : context[match value_of ?FUEL ?EXP ?ENV with Some _ => _ | None => _ end] |- _ ] => destruct (value_of FUEL EXP ENV) eqn:?; try discriminate
+                    | [ _ : context[match ?VAL with Num _ => _ | Bool _ => _ | Clo _ _ _ => _ end] |- _ ] => destruct VAL; try discriminate
+                    | [ _ : context[if ?B then _ else _] |- _ ] => destruct B
+                    | [ H : Some _ = Some _ |- _ ] => inversion H; subst; clear H
+                    end;
+                eauto).
+    Qed.
+
+    Lemma fuel_order : forall ctx (exp : expression ctx) env val fuel fuel', value_of fuel exp env = Some val -> fuel <= fuel' -> value_of fuel' exp env = Some val.
+        Hint Resolve fuel_incr.
+        induction 2; auto.
+    Qed.
+
+    Lemma le_max_1 : forall a b c, a <= max (max a b) c.
+        intros.
+        assert (max a (max b c) = max (max a b) c).
+        apply max_assoc.
+        rewrite <- H.
+        apply le_max_l.
+   Qed.
+
+    Lemma le_max_2 : forall a b c, b <= max (max a b) c.
+        intros.
+        assert (b <= max a b).
+        apply le_max_r.
+        assert (max a b <= max (max a b) c).
+        apply le_max_l.
+        omega.
+    Qed.
+
+    Lemma le_max_3 : forall a b c, c <= max (max a b) c.
+        intros.
+        apply le_max_r.
+    Qed.
+
+    Theorem value_of_completeness : forall ctx (exp : expression ctx) env val, value_of_rel exp env val -> exists fuel, value_of fuel exp env = Some val.
+        Hint Resolve fuel_order le_max_l le_max_r le_max_1 le_max_2 le_max_3.
+        induction 1;
+        match goal with
+        | [ IH1 : exists _, _, IH2 : exists _, _, IH3 : exists _, _ |- _ ] => destruct IH1 as [ fuel1 ? ]; destruct IH2 as [ fuel2 ? ]; destruct IH3 as [ fuel3 ? ]; exists (S (max (max fuel1 fuel2) fuel3))
+        | [ IH1 : exists _, _, IH2 : exists _, _ |- _ ] => destruct IH1 as [ fuel1 ? ]; destruct IH2 as [ fuel2 ? ]; exists (S (max fuel1 fuel2))
+        | [ IH1 : exists _, _ |- _ ] => destruct IH1 as [ fuel1 ? ]; exists (S fuel1)
+        | [ |- _ ] => exists (S O)
+        end;
+        eauto.
+    Qed.
+
+    Theorem value_of_correctness : forall ctx (exp : expression ctx) env val, (exists fuel, value_of fuel exp env = Some val) <-> value_of_rel exp env val.
+        Hint Resolve value_of_soundness value_of_completeness.
+        intros; split; auto.
+    Qed.
 End Lexical.
 
 Module Translation.
-  Definition static_environment := list string.
-  Definition empty_senv : static_environment := nil.
-  Definition extend_senv (x : string) (senv : static_environment) : static_environment := x :: senv.
+    Definition static_environment := list string.
+    Definition empty_senv : static_environment := nil.
+    Definition extend_senv (x : string) (senv : static_environment) : static_environment := x :: senv.
 
-  Fixpoint find_index (x : string) (senv : static_environment) : option nat :=
-      match senv with
-      | nil => None
-      | y :: saved_senv =>
-              if string_dec x y then
-                  Some O
-              else
-                  n <- find_index x saved_senv;
-                  Some (S n)
-      end.
+    Lemma find_index_lemma1 : forall y (saved_senv : static_environment), O < length (y :: saved_senv).
+        intros.
+        simpl.
+        omega.
+    Qed.
 
-  Fixpoint translation_of (exp : Proc.expression) (senv : static_environment) : option Lexical.expression :=
-      match exp with
-      | Proc.Const num => Some (Lexical.Const num)
-      | Proc.Diff exp1 exp2 =>
-              exp1 <- translation_of exp1 senv;
-              exp2 <- translation_of exp2 senv;
-              Some (Lexical.Diff exp1 exp2)
-      | Proc.IsZero exp1 =>
-              exp1 <- translation_of exp1 senv;
-              Some (Lexical.IsZero exp1)
-      | Proc.If exp1 exp2 exp3 =>
-              exp1 <- translation_of exp1 senv;
-              exp2 <- translation_of exp2 senv;
-              exp3 <- translation_of exp3 senv;
-              Some (Lexical.If exp1 exp2 exp3)
-      | Proc.Var var =>
-              n <- find_index var senv;
-              Some (Lexical.Var n)
-      | Proc.Let var exp1 body =>
-              exp1 <- translation_of exp1 senv;
-              body <- translation_of body (extend_senv var senv);
-              Some (Lexical.Let exp1 body)
-      | Proc.Proc var body =>
-              body <- translation_of body (extend_senv var senv);
-              Some (Lexical.Proc body)
-      | Proc.Call rator rand =>
-              rator <- translation_of rator senv;
-              rand <- translation_of rand senv;
-              Some (Lexical.Call rator rand)
-      end.
+    Lemma find_index_lemma2 : forall n y (saved_senv : static_environment), n < length saved_senv -> (S n) < length (y :: saved_senv).
+        intros.
+        simpl.
+        omega.
+    Qed.
 
-  Fixpoint proc_environment_to_static_environment (env : Proc.environment) : static_environment :=
-      match env with
-      | nil => nil
-      | (x, _) :: saved_env => x :: proc_environment_to_static_environment saved_env
-      end.
+    Fixpoint find_index (x : string) (senv : static_environment) : option { n : nat | n < length senv } :=
+        match senv with
+        | nil => None
+        | y :: saved_senv =>
+                if string_dec x y then
+                    Some (exist _ O (find_index_lemma1 _ _))
+                else
+                    res <- find_index x saved_senv;
+                    match res with
+                    | exist n pf => Some (exist _ (S n) (find_index_lemma2 _ _ pf))
+                    end
+        end.
 
-  Fixpoint translation_of_expval (val : Proc.expval) : option Lexical.expval :=
-      match val with
-      | Proc.Num num => Some (Lexical.Num num)
-      | Proc.Bool bool => Some (Lexical.Bool bool)
-      | Proc.Clo var body saved_env =>
-              body <- translation_of body (extend_senv var (proc_environment_to_static_environment saved_env));
-              saved_env <- fold_right (fun pair env =>
-                                           val <- translation_of_expval (snd pair);
-                                           env <- env;
-                                           Some (val :: env)) (Some nil) saved_env;
-              Some (Lexical.Clo body saved_env)
-      end.
+    Fixpoint translation_of (exp : Proc.expression) (senv : static_environment) : option (Lexical.expression (length senv)) :=
+        match exp with
+        | Proc.Const num => Some (Lexical.Const _ num)
+        | Proc.Diff exp1 exp2 =>
+                exp1 <- translation_of exp1 senv;
+                exp2 <- translation_of exp2 senv;
+                Some (Lexical.Diff exp1 exp2)
+        | Proc.IsZero exp1 =>
+                exp1 <- translation_of exp1 senv;
+                Some (Lexical.IsZero exp1)
+        | Proc.If exp1 exp2 exp3 =>
+                exp1 <- translation_of exp1 senv;
+                exp2 <- translation_of exp2 senv;
+                exp3 <- translation_of exp3 senv;
+                Some (Lexical.If exp1 exp2 exp3)
+        | Proc.Var var =>
+                res <- find_index var senv;
+                match res with
+                | exist _ pf => Some (Lexical.Var pf)
+                end
+        | Proc.Let var exp1 body =>
+                exp1 <- translation_of exp1 senv;
+                body <- translation_of body (extend_senv var senv);
+                Some (Lexical.Let exp1 body)
+        | Proc.Proc var body =>
+                body <- translation_of body (extend_senv var senv);
+                Some (Lexical.Proc body)
+        | Proc.Call rator rand =>
+                rator <- translation_of rator senv;
+                rand <- translation_of rand senv;
+                Some (Lexical.Call rator rand)
+        end.
 
-  Definition translation_of_environment (env : Proc.environment) : option Lexical.environment := fold_right (fun pair env =>
-                                val <- translation_of_expval (snd pair);
-                                env <- env;
-                                Some (val :: env)) (Some nil) env.
+    Lemma tranlation_of_const_equation : forall exp senv num, translation_of exp senv = Some (Lexical.Const (length senv) num) -> exp = Proc.Const num.
+        intros.
+        destruct exp; simpl in H;
+        repeat (try match goal with
+                    | [ _ : context[match translation_of ?EXP ?SENV with Some _ => _ | None => _ end] |- _ ] => destruct (translation_of EXP SENV); try discriminate
+                    | [ _ : context[match find_index ?VAR ?SENV with Some _ => _ | None => _ end] |- _ ] => destruct (find_index VAR SENV); try discriminate
+                    | [ H : Some _ = Some _ |- _ ] => inversion H
+                    end;
+                auto).
+        destruct s0.
+        inversion H.
+    Qed.
 
-  Hint Constructors Proc.value_of_rel Lexical.value_of_rel.
+    Lemma translation_of_diff_equation : forall exp senv exp1' exp2', translation_of exp senv = Some (Lexical.Diff exp1' exp2') -> exists exp1 exp2, translation_of exp1 senv = Some exp1' /\ translation_of exp2 senv = Some exp2' /\ exp = Proc.Diff exp1 exp2.
+        intros.
+        Hint Resolve eq_nat_dec.
+        destruct exp; simpl in H;
+        repeat (try match goal with
+                    | [ _ : context[match translation_of ?EXP ?SENV with Some _ => _ | None => _ end] |- _ ] => destruct (translation_of EXP SENV) eqn:?; try discriminate
+                    | [ _ : context[match find_index ?VAR ?SENV with Some _ => _ | None => _ end] |- _ ] => destruct (find_index VAR SENV) eqn:?; try discriminate
+                    | [ H : Some _ = Some _ |- _ ] => inversion H; subst; clear H
+                    | [ H : existT _ _ _ = existT _ _ _ |- _ ] => apply inj_pair2_eq_dec in H; auto; subst
+                    end;
+                eauto).
+        destruct s0.
+        inversion H.
+    Qed.
 
-  Lemma translation_of_soundness_generalized : forall exp exp' env env' val val' senv, translation_of exp senv = Some exp' -> translation_of_environment env = Some env' -> translation_of_expval val = Some val' -> proc_environment_to_static_environment env = senv -> Lexical.value_of_rel exp' env' val' -> Proc.value_of_rel exp env val.
-  Admitted.
+    Lemma translation_of_var_equation : forall exp senv n (pf : n < length senv), translation_of exp senv = Some (Lexical.Var pf) -> exists var pf', find_index var senv = Some (exist _ n pf')  /\ exp = Proc.Var var.
+        intros.
+        Hint Resolve eq_nat_dec.
+        destruct exp; simpl in H;
+        repeat (try match goal with
+                    | [ _ : context[match translation_of ?EXP ?SENV with Some _ => _ | None => _ end] |- _ ] => destruct (translation_of EXP SENV) eqn:?; try discriminate
+                    | [ _ : context[match find_index ?VAR ?SENV with Some _ => _ | None => _ end] |- _ ] => destruct (find_index VAR SENV) eqn:?; try discriminate
+                    | [ H : Some _ = Some _ |- _ ] => inversion H; subst; clear H
+                    | [ H : existT _ _ _ = existT _ _ _ |- _ ] => apply inj_pair2_eq_dec in H; auto; subst
+                    end;
+                eauto).
+        destruct s0.
+        inversion H.
+        subst.
+        eauto.
+    Qed.
 
-  Theorem translation_of_soundness : forall exp exp' val val', translation_of exp empty_senv = Some exp' -> translation_of_expval val = Some val' -> Lexical.value_of_rel exp' Lexical.empty_env val' -> Proc.value_of_rel exp Proc.empty_env val.
-      intros; eapply translation_of_soundness_generalized; eauto; auto.
-  Qed.
+    Fixpoint proc_environment_to_static_environment (env : Proc.environment) : static_environment :=
+        match env with
+        | Proc.Empty => nil
+        | Proc.Extend x _ saved_env => x :: proc_environment_to_static_environment saved_env
+        end.
 
-  Lemma translation_of_completeness_generalized : forall exp exp' env env' val val' senv, translation_of exp senv = Some exp' -> translation_of_environment env = Some env' -> translation_of_expval val = Some val' -> Proc.value_of_rel exp env val -> Lexical.value_of_rel exp' env' val'.
-  Admitted.
+    Fixpoint length_proc_environment (env : Proc.environment) : nat :=
+        match env with
+        | Proc.Empty => O
+        | Proc.Extend _ _ saved_env => S (length_proc_environment saved_env)
+        end.
 
-  Theorem translation_of_completeness : forall exp exp' val val', translation_of exp empty_senv = Some exp' -> translation_of_expval val = Some val' -> Proc.value_of_rel exp Proc.empty_env val -> Lexical.value_of_rel exp' Lexical.empty_env val'.
-      intros; eapply translation_of_completeness_generalized; eauto; auto.
-  Qed.
+    Fixpoint translation_of_expval (val : Proc.expval) : option Lexical.expval :=
+        match val with
+        | Proc.Num num => Some (Lexical.Num num)
+        | Proc.Bool bool => Some (Lexical.Bool bool)
+        | Proc.Clo var body saved_env =>
+                body <- translation_of body (extend_senv var (proc_environment_to_static_environment saved_env));
+                saved_env <- translation_of_environment saved_env;
+                Some (Lexical.Clo body saved_env)
+        end
+
+    with translation_of_environment (env : Proc.environment) : option (Lexical.environment (length (proc_environment_to_static_environment env))) :=
+        match env with
+        | Proc.Empty => Some Lexical.Empty
+        | Proc.Extend _ val saved_env =>
+                val <- translation_of_expval val;
+                saved_env <- translation_of_environment saved_env;
+                Some (Lexical.Extend val saved_env)
+        end.
+
+    Hint Constructors Proc.value_of_rel Lexical.value_of_rel.
+    Hint Constructors Lexical.exp_equiv Lexical.expval_equiv Lexical.env_equiv.
+    Hint Resolve Lexical.exp_equiv_refl Lexical.expval_equiv_refl Lexical.env_equiv_refl.
+
+    Lemma translation_of_expval_inversion_num : forall val num, translation_of_expval val = Some (Lexical.Num num) -> val = Proc.Num num.
+        intros.
+        destruct val.
+            simpl in H.
+            inversion H.
+            trivial.
+
+            simpl in H.
+            inversion H.
+
+            simpl in H.
+            repeat (
+                match goal with
+                | [ _ : context[translation_of ?EXP ?SENV] |- _ ] => destruct (translation_of EXP SENV); try discriminate
+                | [ _ : context[translation_of_environment ?ENV] |- _ ] => destruct (translation_of_environment ENV); try discriminate
+                end).
+    Qed.
+
+    Lemma translation_of_expval_inversion_bool : forall val bool, translation_of_expval val = Some (Lexical.Bool bool) -> val = Proc.Bool bool.
+        intros.
+        destruct val.
+            simpl in H.
+            inversion H.
+
+            simpl in H.
+            inversion H.
+            trivial.
+
+            simpl in H.
+            repeat (
+                match goal with
+                | [ _ : context[translation_of ?EXP ?SENV] |- _ ] => destruct (translation_of EXP SENV); try discriminate
+                | [ _ : context[translation_of_environment ?ENV] |- _ ] => destruct (translation_of_environment ENV); try discriminate
+                end).
+    Qed.
+
+    Lemma translation_of_expval_inversion_clo : forall val ctx (body' : Lexical.expression (S ctx)) saved_env', translation_of_expval val = Some (Lexical.Clo body' saved_env') -> exists var body saved_env bodyt saved_envt, val = Proc.Clo var body saved_env /\ translation_of_environment saved_env = Some saved_envt /\ Lexical.env_equiv saved_envt saved_env' /\ translation_of body (extend_senv var (proc_environment_to_static_environment saved_env)) = Some bodyt /\ Lexical.exp_equiv bodyt body'.
+        intros.
+    Admitted.
+
+    Lemma var_in_environment : forall env s env' x (pf : x < length (proc_environment_to_static_environment env)) (pf' : x < length (proc_environment_to_static_environment env)) val', Lexical.nth env' pf = val' -> find_index s (proc_environment_to_static_environment env) = Some (exist _ x pf') -> translation_of_environment env = Some env' -> exists val valt, translation_of_expval val = Some valt /\ Lexical.expval_equiv valt val' /\ Proc.assoc_error s env = Some val.
+        intros.
+    Admitted.
+
+    Lemma translation_of_soundness_generalized : forall exp env ctx' env' (exp' : Lexical.expression ctx') val' expt envt, translation_of exp (proc_environment_to_static_environment env) = Some expt -> Lexical.exp_equiv expt exp' -> translation_of_environment env = Some envt -> Lexical.env_equiv envt env' -> Lexical.value_of_rel exp' env' val' -> exists val valt, translation_of_expval val = Some valt /\ Lexical.expval_equiv valt val' /\ Proc.value_of_rel exp env val.
+        intros.
+        generalize dependent exp.
+        generalize dependent env.
+        induction H3; intros.
+
+        apply Lexical.exp_equiv_const_inversion in H0.
+        destruct H0.
+        destruct H0.
+        destruct H3.
+        subst.
+        apply tranlation_of_const_equation in H.
+        subst.
+        exists (Proc.Num (Z.of_nat num)).
+        exists (Lexical.Num (Z.of_nat num)).
+        auto.
+
+        apply Lexical.exp_equiv_diff_inversion in H0.
+        destruct H0.
+        destruct H0.
+        destruct H0.
+        destruct H3.
+        subst.
+        apply translation_of_diff_equation in H.
+        destruct H.
+        destruct H.
+        destruct H.
+        destruct H4.
+        subst.
+        assert (T1 := IHvalue_of_rel1 env0 x envt).
+        eapply T1 in H0; eauto.
+        destruct H0.
+        destruct H0.
+        destruct H0.
+        destruct H5.
+        subst.
+        inversion H5.
+        subst.
+        apply translation_of_expval_inversion_num in H0.
+        subst.
+        assert (T2 := IHvalue_of_rel2 env0 x0 envt).
+        eapply T2 in H3; eauto.
+        destruct H3.
+        destruct H0.
+        destruct H0.
+        destruct H3.
+        subst.
+        inversion H3.
+        subst.
+        apply translation_of_expval_inversion_num in H0.
+        subst.
+        exists (Proc.Num (num1 - num2)).
+        exists (Lexical.Num (num1 - num2)).
+        auto.
+
+        admit.
+
+        admit.
+
+        admit.
+
+        apply Lexical.exp_equiv_var_inversion in H0.
+        destruct H0.
+        destruct H0.
+        destruct H0.
+        destruct H4.
+        subst.
+        apply translation_of_var_equation in H3.
+        destruct H3.
+        destruct H.
+        destruct H.
+        subst.
+        assert (Lexical.nth envt pf = Lexical.nth envt pf).
+        trivial.
+        apply var_in_environment with (s := x) (pf' := x1) in H0; auto.
+        admit.
+
+        admit.
+
+        admit.
+    Admitted.
+
+    Theorem translation_of_soundness : forall exp exp' val', translation_of exp empty_senv = Some exp' -> Lexical.value_of_rel exp' Lexical.Empty val' -> exists val valt, translation_of_expval val = Some valt /\ Lexical.expval_equiv valt val' /\ Proc.value_of_rel exp Proc.Empty val.
+        intros; eapply translation_of_soundness_generalized; eauto; auto.
+    Qed.
+
+    Lemma translation_of_completeness_generalized : forall env env' exp exp' val val', translation_of exp (proc_environment_to_static_environment env) = Some exp' -> translation_of_environment env = Some env' -> translation_of_expval val = Some val' -> Proc.value_of_rel exp env val -> Lexical.value_of_rel exp' env' val'.
+    Admitted.
+
+    Theorem translation_of_completeness : forall exp exp' val val', translation_of exp (proc_environment_to_static_environment Proc.Empty) = Some exp' -> translation_of_expval val = Some val' -> Proc.value_of_rel exp Proc.Empty val -> Lexical.value_of_rel exp' Lexical.Empty val'.
+        intros; eapply translation_of_completeness_generalized; eauto; auto.
+    Qed.
 End Translation.
